eIris/proofmode/startProof.v
@@ -4,15 +4,18 @@ From iris.prelude Require Import options.
 
 From eIris.proofmode Require Import base.
 From eIris.common Extra Dependency "stdpp.elpi" as stdpp.
+From eIris.common Extra Dependency "tokenize.elpi" as tokenize.
+From eIris.common Extra Dependency "parser.elpi" as parser.
 From eIris.proofmode.elpi Extra Dependency "iris_ltac.elpi" as iris_ltac.
 From eIris.proofmode.elpi Extra Dependency "eiris_tactics.elpi" as eiris_tactics.
 
 From iris.heap_lang Require Import proofmode.
  
 Elpi Tactic eiStartProof.
-
 Elpi Accumulate File stdpp.
 Elpi Accumulate File iris_ltac.
+Elpi Accumulate File tokenize.
+Elpi Accumulate File parser.
 Elpi Accumulate File eiris_tactics.
 Elpi Accumulate lp:{{
   solve G GL :-
