eIris/tests/test_elpi.v
@@ -2,7 +2,7 @@ From elpi Require Import elpi.
 From iris.proofmode Require Export tactics coq_tactics reduction.
 From iris.prelude Require Import options.
 From iris.heap_lang Require Import proofmode.
-(* From eIris.proofmode Require Import split. *)
+From eIris.proofmode Require Import split.
 
 Elpi Tactic print_args.
 Elpi Accumulate lp:{{
