eIris/tests/twp.v
@@ -1,0 +1,31 @@
+From iris.bi Require Import fixpoint big_op.
+From iris.proofmode Require Import proofmode.
+From iris.program_logic Require Export weakestpre.
+From iris.prelude Require Import options.
+
+From eIris.proofmode Require Import inductive.
+
+Section TWP.
+
+  Context `{!irisGS_gen hlc Λ Σ}.
+
+  EI.ind 
+  Inductive twp2 : coPset -> expr Λ -> (val Λ → iProp Σ) -> iProp Σ :=
+    twp2_some : |={E}=> Φ v -∗ twp2 E (Some v) Φ.
+
+  Definition twp_pre `{!irisGS_gen hlc Λ Σ} (s : stuckness)
+      (wp : coPset → expr Λ → (val Λ → iProp Σ) → iProp Σ) :
+    coPset → expr Λ → (val Λ → iProp Σ) → iProp Σ := λ E e1 Φ,
+  match to_val e1 with
+  | Some v => |={E}=> Φ v
+  | None => ∀ σ1 ns κs nt,
+     state_interp σ1 ns κs nt ={E,∅}=∗
+       ⌜if s is NotStuck then reducible_no_obs e1 σ1 else True⌝ ∗
+       ∀ κ e2 σ2 efs, ⌜prim_step e1 σ1 κ e2 σ2 efs⌝ ={∅,E}=∗
+         ⌜κ = []⌝ ∗
+         state_interp σ2 (S ns) κs (length efs + nt) ∗
+         wp E e2 Φ ∗
+         [∗ list] ef ∈ efs, wp ⊤ ef fork_post
+  end%I.
+
+End TWP.
